imports.v
@@ -3,5 +3,7 @@ From Coq Require Export Logic.PropExtensionality
   (propositional_extensionality) Program.Basics (const).
 From Equations Require Export Equations.
 From Hammer Require Export Tactics.
-From stdpp Require Export relations (rtc, rtc_transitive, rtc_once, rtc_inv, rtc(..), diamond, confluent, diamond_confluent).
+From stdpp Require Export relations (rtc, rtc_transitive, rtc_once, rtc_inv, rtc(..), diamond, confluent, diamond_confluent) option (from_option).
+
 Require Export Psatz.
+From HB Require Export structures.
